removed role from Fam

src/FcEtt/ett_ott.v
@@ -24,7 +24,7 @@ with tm : Set :=  (*r types and kinds *)
  | a_Abs (rho:relflag) (A:tm) (R:role) (b:tm)
  | a_UAbs (rho:relflag) (R:role) (b:tm)
  | a_App (a:tm) (rho:relflag) (R:role) (b:tm)
- | a_Fam (F:tyfam) (R:role)
+ | a_Fam (F:tyfam)
  | a_Const (T:const)
  | a_Pi (rho:relflag) (A:tm) (R:role) (B:tm)
  | a_Conv (a:tm) (R:role) (g:co)
@@ -136,7 +136,7 @@ with open_tm_wrt_co_rec (k:nat) (g5:co) (a5:tm) {struct a5}: tm :=
   | (a_Abs rho A R b) => a_Abs rho (open_tm_wrt_co_rec k g5 A) R (open_tm_wrt_co_rec k g5 b)
   | (a_UAbs rho R b) => a_UAbs rho R (open_tm_wrt_co_rec k g5 b)
   | (a_App a rho R b) => a_App (open_tm_wrt_co_rec k g5 a) rho R (open_tm_wrt_co_rec k g5 b)
-  | (a_Fam F R) => a_Fam F R
+  | (a_Fam F) => a_Fam F
   | (a_Const T) => a_Const T
   | (a_Pi rho A R B) => a_Pi rho (open_tm_wrt_co_rec k g5 A) R (open_tm_wrt_co_rec k g5 B)
   | (a_Conv a R g) => a_Conv (open_tm_wrt_co_rec k g5 a) R (open_co_wrt_co_rec k g5 g)
@@ -201,7 +201,7 @@ with open_tm_wrt_tm_rec (k:nat) (a5:tm) (a_6:tm) {struct a_6}: tm :=
   | (a_Abs rho A R b) => a_Abs rho (open_tm_wrt_tm_rec k a5 A) R (open_tm_wrt_tm_rec (S k) a5 b)
   | (a_UAbs rho R b) => a_UAbs rho R (open_tm_wrt_tm_rec (S k) a5 b)
   | (a_App a rho R b) => a_App (open_tm_wrt_tm_rec k a5 a) rho R (open_tm_wrt_tm_rec k a5 b)
-  | (a_Fam F R) => a_Fam F R
+  | (a_Fam F) => a_Fam F
   | (a_Const T) => a_Const T
   | (a_Pi rho A R B) => a_Pi rho (open_tm_wrt_tm_rec k a5 A) R (open_tm_wrt_tm_rec (S k) a5 B)
   | (a_Conv a R g) => a_Conv (open_tm_wrt_tm_rec k a5 a) R (open_co_wrt_tm_rec k a5 g)
@@ -390,8 +390,8 @@ with lc_tm : tm -> Prop :=    (* defn lc_tm *)
      (lc_tm a) ->
      (lc_tm b) ->
      (lc_tm (a_App a rho R b))
- | lc_a_Fam : forall (F:tyfam) (R:role),
-     (lc_tm (a_Fam F R))
+ | lc_a_Fam : forall (F:tyfam),
+     (lc_tm (a_Fam F))
  | lc_a_Const : forall (T:const),
      (lc_tm (a_Const T))
  | lc_a_Pi : forall (rho:relflag) (A:tm) (R:role) (B:tm),
@@ -496,7 +496,7 @@ with fv_tm_tm_tm (a5:tm) : vars :=
   | (a_Abs rho A R b) => (fv_tm_tm_tm A) \u (fv_tm_tm_tm b)
   | (a_UAbs rho R b) => (fv_tm_tm_tm b)
   | (a_App a rho R b) => (fv_tm_tm_tm a) \u (fv_tm_tm_tm b)
-  | (a_Fam F R) => {}
+  | (a_Fam F) => {}
   | (a_Const T) => {}
   | (a_Pi rho A R B) => (fv_tm_tm_tm A) \u (fv_tm_tm_tm B)
   | (a_Conv a R g) => (fv_tm_tm_tm a) \u (fv_tm_tm_co g)
@@ -556,7 +556,7 @@ with fv_co_co_tm (a5:tm) : vars :=
   | (a_Abs rho A R b) => (fv_co_co_tm A) \u (fv_co_co_tm b)
   | (a_UAbs rho R b) => (fv_co_co_tm b)
   | (a_App a rho R b) => (fv_co_co_tm a) \u (fv_co_co_tm b)
-  | (a_Fam F R) => {}
+  | (a_Fam F) => {}
   | (a_Const T) => {}
   | (a_Pi rho A R B) => (fv_co_co_tm A) \u (fv_co_co_tm B)
   | (a_Conv a R g) => (fv_co_co_tm a) \u (fv_co_co_co g)
@@ -641,7 +641,7 @@ with tm_subst_tm_tm (a5:tm) (x5:tmvar) (a_6:tm) {struct a_6} : tm :=
   | (a_Abs rho A R b) => a_Abs rho (tm_subst_tm_tm a5 x5 A) R (tm_subst_tm_tm a5 x5 b)
   | (a_UAbs rho R b) => a_UAbs rho R (tm_subst_tm_tm a5 x5 b)
   | (a_App a rho R b) => a_App (tm_subst_tm_tm a5 x5 a) rho R (tm_subst_tm_tm a5 x5 b)
-  | (a_Fam F R) => a_Fam F R
+  | (a_Fam F) => a_Fam F
   | (a_Const T) => a_Const T
   | (a_Pi rho A R B) => a_Pi rho (tm_subst_tm_tm a5 x5 A) R (tm_subst_tm_tm a5 x5 B)
   | (a_Conv a R g) => a_Conv (tm_subst_tm_tm a5 x5 a) R (tm_subst_tm_co a5 x5 g)
@@ -701,7 +701,7 @@ with co_subst_co_tm (g5:co) (c5:covar) (a5:tm) {struct a5} : tm :=
   | (a_Abs rho A R b) => a_Abs rho (co_subst_co_tm g5 c5 A) R (co_subst_co_tm g5 c5 b)
   | (a_UAbs rho R b) => a_UAbs rho R (co_subst_co_tm g5 c5 b)
   | (a_App a rho R b) => a_App (co_subst_co_tm g5 c5 a) rho R (co_subst_co_tm g5 c5 b)
-  | (a_Fam F R) => a_Fam F R
+  | (a_Fam F) => a_Fam F
   | (a_Const T) => a_Const T
   | (a_Pi rho A R B) => a_Pi rho (co_subst_co_tm g5 c5 A) R (co_subst_co_tm g5 c5 B)
   | (a_Conv a R g) => a_Conv (co_subst_co_tm g5 c5 a) R (co_subst_co_co g5 c5 g)
@@ -768,7 +768,7 @@ Fixpoint erase_tm (a : tm) (r : role) : tm :=
    | a_App a Rel R b => a_App (erase_tm a r) Rel R (erase_tm b R)
    | a_App a Irrel R b => a_App (erase_tm a r) Irrel R a_Bullet
    | a_Const T => a_Const T
-   | a_Fam F R => a_Fam F R
+   | a_Fam F => a_Fam F
    | a_Pi rho A R B => a_Pi rho (erase_tm A R) R (erase_tm B r)
    | a_Conv a r1 g => if (lte_role r1 r) then
 	                      erase_tm a r else
@@ -818,7 +818,7 @@ Definition FixDef : tm :=
   (a_Abs Irrel a_Star Nom
          (a_Abs Rel (a_Pi Rel (a_Var_b 0) Nom (a_Var_b 1)) Nom
                 (a_App (a_Var_b 0) Rel Nom
-                       (a_App (a_App (a_Fam Fix Nom) Irrel Nom (a_Var_b 1)) Rel Nom (a_Var_b 0))))).
+                       (a_App (a_App (a_Fam Fix) Irrel Nom (a_Var_b 1)) Rel Nom (a_Var_b 0))))).
 
 Definition FixTy : tm :=
   a_Pi Irrel a_Star Nom
@@ -894,10 +894,10 @@ with Value : role -> tm -> Prop :=    (* defn Value *)
  | Value_UCAbs : forall (R:role) (a:tm),
      lc_tm (a_UCAbs a) ->
      Value R (a_UCAbs a)
- | Value_Ax : forall (R:role) (F:tyfam) (R1:role) (a A:tm),
+ | Value_Ax : forall (R:role) (F:tyfam) (a A:tm) (R1:role),
       binds  F  (Ax  a A R1 )   toplevel   ->
       not (  ( SubRole R1 R )  )  ->
-     Value R  ( (a_Fam F R1) ) 
+     Value R (a_Fam F)
 with value_type : role -> tm -> Prop :=    (* defn value_type *)
  | value_type_Star : forall (R:role),
      value_type R a_Star
@@ -909,10 +909,10 @@ with value_type : role -> tm -> Prop :=    (* defn value_type *)
      lc_constraint phi ->
      lc_tm (a_CPi phi B) ->
      value_type R (a_CPi phi B)
- | value_type_Ax : forall (R:role) (F:tyfam) (R1:role) (a A:tm),
+ | value_type_Ax : forall (R:role) (F:tyfam) (a A:tm) (R1:role),
       binds  F  (Ax  a A R1 )   toplevel   ->
       not (  ( SubRole R1 R )  )  ->
-     value_type R  ( (a_Fam F R1) ) .
+     value_type R (a_Fam F).
 
 (* defns Jconsistent *)
 Inductive consistent : tm -> tm -> role -> Prop :=    (* defn consistent *)
@@ -930,8 +930,8 @@ Inductive consistent : tm -> tm -> role -> Prop :=    (* defn consistent *)
      lc_constraint phi2 ->
      lc_tm (a_CPi phi2 A2) ->
      consistent  ( (a_CPi phi1 A1) )   ( (a_CPi phi2 A2) )  R
- | consistent_a_Fam : forall (F:tyfam) (R R':role),
-     consistent  ( (a_Fam F R) )   ( (a_Fam F R) )  R'
+ | consistent_a_Fam : forall (F:tyfam) (R':role),
+     consistent (a_Fam F) (a_Fam F) R'
  | consistent_a_Step_R : forall (a b:tm) (R:role),
      lc_tm a ->
       not ( value_type R b )  ->
@@ -977,11 +977,11 @@ Inductive erased_tm : role_context -> tm -> role -> Prop :=    (* defn erased_tm
  | erased_a_CApp : forall (W:role_context) (a:tm) (R:role),
      erased_tm W a R ->
      erased_tm W  ( (a_CApp a g_Triv) )  R
- | erased_a_Fam : forall (W:role_context) (F:tyfam) (R R1:role) (a A:tm),
+ | erased_a_Fam : forall (W:role_context) (F:tyfam) (R1:role) (a A:tm) (R:role),
       uniq  W  ->
       binds  F  (Ax  a A R )   toplevel   ->
      SubRole R R1 ->
-     erased_tm W  ( (a_Fam F R) )  R1
+     erased_tm W (a_Fam F) R1
  | erased_a_Const : forall (W:role_context) (T:const) (R:role),
       uniq  W  ->
      erased_tm W (a_Const T) R
@@ -1033,11 +1033,11 @@ Inductive Par : context -> available_props -> role_context -> tm -> tm -> role -
      Par G D W b b' R1 ->
       ( forall c , c \notin  L  -> Par G D W  ( open_tm_wrt_co B (g_Var_f c) )   ( open_tm_wrt_co B' (g_Var_f c) )  R )  ->
      Par G D W (a_CPi (Eq a b A R1) B) (a_CPi (Eq a' b' A' R1) B') R
- | Par_Axiom : forall (G:context) (D:available_props) (W:role_context) (F:tyfam) (R1:role) (a:tm) (R:role) (A:tm),
+ | Par_Axiom : forall (G:context) (D:available_props) (W:role_context) (F:tyfam) (a:tm) (R:role) (A:tm) (R1:role),
       binds  F  (Ax  a A R1 )   toplevel   ->
      SubRole R1 R ->
       uniq  W  ->
-     Par G D W  ( (a_Fam F R1) )  a R
+     Par G D W (a_Fam F) a R
  | Par_Cong : forall (G:context) (D:available_props) (W:role_context) (a1:tm) (R:role) (a2:tm) (R1:role),
      Par G D W a1 a2 R1 ->
      Par G D W (a_Conv a1 R g_Triv) (a_Conv a2 R g_Triv) R1
@@ -1078,9 +1078,9 @@ Inductive Beta : tm -> tm -> role -> Prop :=    (* defn Beta *)
  | Beta_CAppCAbs : forall (a':tm) (R:role),
      lc_tm (a_UCAbs a') ->
      Beta (a_CApp  ( (a_UCAbs a') )  g_Triv)  (open_tm_wrt_co  a'   g_Triv )  R
- | Beta_Axiom : forall (F:tyfam) (R:role) (a A:tm),
+ | Beta_Axiom : forall (F:tyfam) (a:tm) (R:role) (A:tm),
       binds  F  (Ax  a A R )   toplevel   ->
-     Beta  ( (a_Fam F R) )  a R
+     Beta (a_Fam F) a R
 with reduction_in_one : tm -> tm -> role -> Prop :=    (* defn reduction_in_one *)
  | E_AbsTerm : forall (L:vars) (R:role) (a a':tm) (R1:role),
       ( forall x , x \notin  L  -> reduction_in_one  ( open_tm_wrt_tm a (a_Var_f x) )   ( open_tm_wrt_tm a' (a_Var_f x) )  R1 )  ->
@@ -1099,10 +1099,10 @@ with reduction_in_one : tm -> tm -> role -> Prop :=    (* defn reduction_in_one 
  | E_CAppCAbs : forall (b:tm) (R:role),
      lc_tm (a_UCAbs b) ->
      reduction_in_one (a_CApp  ( (a_UCAbs b) )  g_Triv)  (open_tm_wrt_co  b   g_Triv )  R
- | E_Axiom : forall (F:tyfam) (R:role) (a:tm) (R1:role) (A:tm),
+ | E_Axiom : forall (F:tyfam) (a:tm) (R1:role) (A:tm) (R:role),
       binds  F  (Ax  a A R )   toplevel   ->
      SubRole R R1 ->
-     reduction_in_one  ( (a_Fam F R) )  a R1
+     reduction_in_one (a_Fam F) a R1
  | E_Cong : forall (a:tm) (R:role) (a':tm) (R1:role),
      reduction_in_one a a' R1 ->
       not (  ( SubRole R R1 )  )  ->
@@ -1181,11 +1181,11 @@ with Typing : context -> tm -> tm -> role -> Prop :=    (* defn Typing *)
      Typing G a1 (a_CPi  ( (Eq a b A R) )  B1) R' ->
      DefEq G  (dom  G )  a b A R ->
      Typing G (a_CApp a1 g_Triv)  (open_tm_wrt_co  B1   g_Triv )  R'
- | E_Fam : forall (G:context) (F:tyfam) (R:role) (A a:tm),
+ | E_Fam : forall (G:context) (F:tyfam) (A:tm) (R:role) (a:tm),
      Ctx G ->
       binds  F  (Ax  a A R )   toplevel   ->
       ( Typing  nil  A a_Star R )  ->
-     Typing G  ( (a_Fam F R) )  A R
+     Typing G (a_Fam F) A R
  | E_TyCast : forall (G:context) (a:tm) (R2:role) (A2:tm) (R1:role) (A1:tm),
      Typing G a A1 R1 ->
      DefEq G  (dom  G )  A1 A2 a_Star R2 ->
@@ -1370,11 +1370,11 @@ with AnnTyping : context -> tm -> tm -> role -> Prop :=    (* defn AnnTyping *)
      AnnTyping G a1  ( (a_CPi (Eq a b A1 R) B) )  R' ->
      AnnDefEq G  (dom  G )  g a b R ->
      AnnTyping G (a_CApp a1 g)  (open_tm_wrt_co  B   g )  R'
- | An_Fam : forall (G:context) (F:tyfam) (R:role) (A a:tm),
+ | An_Fam : forall (G:context) (F:tyfam) (A:tm) (R:role) (a:tm),
      AnnCtx G ->
       binds  F  (Ax  a A R )   an_toplevel   ->
       ( AnnTyping  nil  A a_Star R )  ->
-     AnnTyping G  ( (a_Fam F R) )  A R
+     AnnTyping G (a_Fam F) A R
  | An_SubRole : forall (G:context) (a A:tm) (R2 R1:role),
      SubRole R1 R2 ->
      AnnTyping G a A R1 ->
@@ -1556,9 +1556,9 @@ Inductive head_reduction : context -> tm -> tm -> role -> Prop :=    (* defn hea
      AnnTyping G A a_Star R ->
       ( forall x , x \notin  L  -> head_reduction  (( x ~ Tm  A R ) ++  G )   ( open_tm_wrt_tm b (a_Var_f x) )   ( open_tm_wrt_tm b' (a_Var_f x) )  R1 )  ->
      head_reduction G  ( (a_Abs Irrel A R b) )   ( (a_Abs Irrel A R b') )  R1
- | An_Axiom : forall (G:context) (F:tyfam) (R:role) (a A:tm),
+ | An_Axiom : forall (G:context) (F:tyfam) (a:tm) (R:role) (A:tm),
       binds  F  (Ax  a A R )   an_toplevel   ->
-     head_reduction G  ( (a_Fam F R) )  a R
+     head_reduction G (a_Fam F) a R
  | An_ConvTerm : forall (G:context) (a:tm) (R1:role) (g:co) (a':tm) (R:role),
      lc_co g ->
      head_reduction G a a' R ->
